Instantiate propositional formula encodable

Modallogic/Propositional/Formula.lean
@@ -1,13 +1,16 @@
 import Lean
 import Mathlib.Data.Set.Basic
+import Mathlib.Logic.Encodable.Basic
+
+open Option Nat Encodable
 
 namespace Modallogic
 
 namespace Propositional
 
 inductive Formula (α : Type) : Type
-| var : α → Formula α
 | bot : Formula α
+| var : α → Formula α
 | impl : Formula α → Formula α → Formula α
 
 namespace Formula
@@ -15,6 +18,8 @@ namespace Formula
 prefix:max "#" => var
 notation "⊥ₚ" => bot
 infixr:30 " →ₚ " => impl
+
+section
 
 variable (φ ψ χ : Formula α)
 def not := φ →ₚ ⊥ₚ
@@ -32,16 +37,15 @@ infixl:50 " ∧ₚ " => and
 def iff := (φ →ₚ ψ) ∧ₚ (ψ →ₚ φ)
 infixl:30 " ↔ₚ " => iff
 
-def toString [ToString α] : Formula α → String
-| φ →ₚ ψ => s!"({toString φ} → {toString ψ})"
+end
+
+def toStr [ToString α] : Formula α → String
+| φ →ₚ ψ => s!"({toStr φ} → {toStr ψ})"
 | ⊥ₚ => "⊥"
 | #p => s!"#{p}"
 
-instance [ToString α] : Repr (Formula α) := ⟨λ t _ => Formula.toString t⟩
-
-instance [ToString α] : ToString (Formula α) := ⟨Formula.toString⟩
-
-#eval (#1 →ₚ #2 ∧ₚ #1)
+instance [ToString α] : Repr (Formula α) := ⟨λ t _ => toStr t⟩
+instance [ToString α] : ToString (Formula α) := ⟨toStr⟩
 
 def beq [BEq α] (φ ψ : Formula α) : Bool :=
   match φ, ψ with
@@ -51,14 +55,46 @@ def beq [BEq α] (φ ψ : Formula α) : Bool :=
   | _, _ => false
 instance [BEq α] : BEq (Formula α) := ⟨Formula.beq⟩
 
-#eval (#1 →ₚ #2 →ₚ #1) == (#1 →ₚ (#2 →ₚ #1))
+section
+
+variable [Encodable α]
+
+def toNat : Formula α → ℕ
+  | ⊥ₚ => 0
+  | #p => 2 * (encode p) + 1
+  | φ →ₚ ψ => 2 * (pair (φ.toNat) (ψ.toNat)) + 2
+
+def ofNat : ℕ → Option (Formula α)
+  | 0 => some ⊥ₚ
+  | n + 1 =>
+    match n.bodd with
+    | false => (decode n.div2).map Formula.var
+    | true =>
+      let m := n.div2
+      have h : m < n + 1 := by
+        apply lt_succ_iff.mpr; simp [div2_val]; exact div_le_self n 2;
+      have : (unpair m).1 < n + 1 := lt_of_le_of_lt (unpair_left_le _) h;
+      have : (unpair m).2 < n + 1 := lt_of_le_of_lt (unpair_right_le _) h;
+      let φ := ofNat m.unpair.1
+      let ψ := ofNat m.unpair.2
+      φ.bind (λ φ => ψ.map (λ ψ => φ →ₚ ψ))
+  termination_by ofNat n => n
+
+theorem ofNat_toNat : ∀ (φ : Formula α), ofNat (toNat φ) = some φ
+  | ⊥ₚ => by simp [toNat, ofNat];
+  | #p => by simp [toNat, ofNat, div2_val];
+  | φ →ₚ ψ => by simp [toNat, ofNat, div2_val, ofNat_toNat];
+
+instance : Encodable (Formula α) where
+  encode := toNat
+  decode := ofNat
+  encodek := ofNat_toNat
+
+end
 
 end Formula
 
 abbrev Formulae (α : Type) := Set (Formula α)
-
-def inconsistent (Γ : Formulae α) :=  ∃ φ, (φ ∈ Γ ∧ ¬ₚφ ∈ Γ)
-def consistent (Γ : Formulae α) := ¬(inconsistent Γ)
 
 end Modallogic.Propositional
 
